

Построение сплайна через моменты

Введём обозначения:

$$S''(x_i) = M_i, i = \overline{0, n}$$

$$S(x) = y_i + c_i(x - x_i) + a_i \frac{(x - x_i)^2}{2} + b_i \frac{(x - x_i)^3}{6}, i = \overline{0, n-1}$$

$$S'(x) = c_i + a_i(x - x_i) + b_i \frac{(x - x_i)^2}{2}, i = \overline{0, n-1}$$

$$S''(x) = a_i + b_i(x - x_i), i = \overline{0, n-1}$$

$$S''(x_i) = a_i = M_i, S''(x_{i+1}) = a_i + b_i h_{i+1} = M_{i+1}$$

$$b_i = \frac{M_{i+1} - M_i}{h_{i+1}}$$

$$S(x_{i+1}) = y_i + c_i h_{i+1} + a_i \frac{h_{i+1}^2}{2} + b_i \frac{h_{i+1}^3}{6} = y_{i+1}$$

$$c_i = \frac{y_{i+1} - y_i}{h_{i+1}} - M_i \frac{h_{i+1}^2}{2h_{i+1}} - \frac{(M_{i+1} - M_i)h_{i+1}^3}{h_{i+1}6h_{i+1}}$$

$$c_i = \frac{y_{i+1} - y_i}{h_{i+1}} - \frac{h_{i+1}}{6}(M_{i+1} + 2M_i)$$

$$S'(x) = c_i + a_i(x - x_i) + b_i \frac{(x - x_i)^2}{2}, x \in [x_i; x_{i+1}]$$

$$S'(x) = c_{i-1} + a_{i-1}(x - x_{i-1}) + b_{i-1} \frac{(x - x_{i-1})^2}{2}, x \in [x_{i-1}; x_i]$$

$$S'(x_i - 0) = S'(x_i + 0)$$

$$c_{i-1} + a_{i-1}h_i + b_{i-1} \frac{h_i^2}{2} = c_i$$

$$\frac{y_i - y_{i-1}}{h_i} - \frac{h_i}{6}(M_i + 2M_{i-1}) + M_{i-1}h_i + \frac{M_i - M_{i-1}}{h_i} \frac{h_i^2}{2} = \frac{y_{i+1} - y_i}{h_{i+1}} - \frac{h_{i+1}}{6}(M_{i+1} + 2M_i)$$

$$\frac{h_{i+1}}{6}(M_{i+1} + 2M_i) - \frac{h_i}{6}(M_i + 2M_{i-1}) + M_{i-1}h_i + \frac{h_i}{2}(M_i - M_{i-1}) = \frac{y_{i+1} - y_i}{h_{i+1}} -$$

$$\frac{y_i - y_{i-1}}{h_i} \Bigg| \times 6$$

$$h_i M_{i-1} + 2M_i(h_{i+1} + h_i) + h_{i+1} M_{i+1} = 6 \left(\frac{y_{i+1} - y_i}{h_{i+1}} - \frac{y_i - y_{i-1}}{h_i} \right) \left| \times \frac{1}{h_i + h_{i+1}} \right.$$

$$\mu_i = \frac{h_{i+1}}{h_i + h_{i+1}}; \lambda_i = \frac{h_i}{h_i + h_{i+1}}; \lambda_i + \mu_i = 1$$

$$\lambda_i M_{i-1} + 2M_i + \mu_i M_{i+1} = 6 \underbrace{\left(\mu_i \frac{y_{i+1} - y_i}{h_{i+1}^2} - \lambda_i \frac{y_i - y_{i-1}}{h_i^2} \right)}_{g_i}$$

$$i = \overline{1, n-1}; M_0, M_1, \dots, M_{n-1}, M_n$$

Краевые условия:

$$1) S'(a) = f'(a), S'(b) = f'(b);$$

$$S'(a) = c_0 + a_0(a - x_0) + b_0 \frac{(a - x_0)^2}{2} = c_0 = \frac{y_1 - y_0}{h_1} - \frac{h_1}{6} (M_1 + 2M_0) = f'(a)$$

$$2M_0 + M_1 = 6 \underbrace{\frac{y_1 - y_0}{h_1} - \frac{6}{h_1} f'(a)}_{g_0}$$

$$S'(b) = c_{n-1} + a_{n-1}(b - x_{n-1}) + b_{n-1} \frac{(b - x_{n-1})^2}{2} = c_{n-1} + a_{n-1}h_n + b_{n-1} \frac{h_n^2}{2} =$$

$$\frac{y_n - y_{n-1}}{h_n} - \frac{h_n}{6} (M_n + 2M_{n-1}) + h_n M_{n-1} + \frac{M_n - M_{n-1}}{h_n} \frac{h_n^2}{2} = f'(b)$$

$$M_{n-1} + 2M_n = \underbrace{\frac{6}{h_n} f'(b) - 6 \frac{y_n - y_{n-1}}{h_n^2}}_{g_n}$$

$$\begin{pmatrix} 2 & 1 & 0 & 0 & \cdots & 0 & 0 & 0 \\ \lambda_1 & 2 & \mu_1 & 0 & \cdots & 0 & 0 & 0 \\ 0 & \lambda_2 & 2 & \mu_2 & \cdots & 0 & 0 & 0 \\ \vdots & \vdots & \vdots & \vdots & \ddots & \vdots & \vdots & \vdots \\ 0 & 0 & 0 & 0 & \cdots & \lambda_{n-1} & 2 & \mu_{n-1} \\ 0 & 0 & 0 & 0 & \cdots & 0 & 1 & 2 \end{pmatrix} \begin{pmatrix} M_0 \\ M_1 \\ M_2 \\ \vdots \\ M_{n-1} \\ M_n \end{pmatrix} = \begin{pmatrix} g_0 \\ g_1 \\ g_2 \\ \vdots \\ g_{n-1} \\ g_n \end{pmatrix}$$

$$3) S''(a) = f''(a), S''(b) = f''(b);$$

$$M_0 = f''(a), M_n = f''(b)$$

$$\begin{pmatrix} 1 & 0 & 0 & 0 & \cdots & 0 & 0 & 0 \\ \lambda_1 & 2 & \mu_1 & 0 & \cdots & 0 & 0 & 0 \\ 0 & \lambda_2 & 2 & \mu_2 & \cdots & 0 & 0 & 0 \\ \vdots & \vdots & \vdots & \vdots & \ddots & \vdots & \vdots & \vdots \\ 0 & 0 & 0 & 0 & \cdots & \lambda_{n-1} & 2 & \mu_{n-1} \\ 0 & 0 & 0 & 0 & \cdots & 0 & 0 & 1 \end{pmatrix} \begin{pmatrix} M_0 \\ M_1 \\ M_2 \\ \vdots \\ M_{n-1} \\ M_n \end{pmatrix} = \begin{pmatrix} f''(a) \\ g_1 \\ g_2 \\ \vdots \\ g_{n-1} \\ f''(b) \end{pmatrix}$$

$$5) f(a) = f(b), f(x_{n+1}) = f(x_1), \dots$$

$$M_0 = M_n, M_{n+1} = M_1, \dots$$

$$h_{n+1} = h_1, h_{n+2} = h_2, \dots$$

$$\mu_{n+1} = \mu_1, \dots$$

$$i = 1 :$$

$$\lambda_1 M_0 + 2M_1 + M_2 = g_1$$

$$2M_1 + \mu_1 M_2 + \lambda_1 M_n = g_1$$

$$i = n :$$

$$\lambda_n M_{n-1} + 2M_n + \mu_n M_{n+1} = g_n$$

$$\mu_n M_1 + \lambda_n M_{n-1} + 2M_n = g_n$$

$$\begin{pmatrix} 2 & \mu_1 & 0 & 0 & \cdots & 0 & 0 & \lambda_1 \\ \lambda_2 & 2 & \mu_2 & 0 & \cdots & 0 & 0 & 0 \\ 0 & \lambda_3 & 2 & \mu_3 & \cdots & 0 & 0 & 0 \\ \vdots & \vdots & \vdots & \vdots & \ddots & \vdots & \vdots & \vdots \\ 0 & 0 & 0 & 0 & \cdots & \lambda_{n-1} & 2 & \mu_{n-1} \\ \mu_n & 0 & 0 & 0 & \cdots & 0 & \lambda_n & 2 \end{pmatrix} \begin{pmatrix} M_1 \\ M_2 \\ M_3 \\ \vdots \\ M_{n-1} \\ M_n \end{pmatrix} = \begin{pmatrix} g_1 \\ g_2 \\ g_3 \\ \vdots \\ g_{n-1} \\ g_n \end{pmatrix}$$

$$6) S'''(x_1 + 0) = S'''(x_1 - 0), S'''(x_{n-1} + 0) = S'''(x_{n-1} - 0);$$

$$S'''(x) = b_i, x \in [x_i, x_{i+1}]$$

$$\begin{aligned}
b_0 &= b_1 \\
\frac{M_1 - M_0}{h_1} &= \frac{M_2 - M_1}{h_2} \Big| \times h_1 \\
\gamma_1 &= \frac{h_1}{h_2} \\
M_0 - M_1(1 + \gamma_1) + \gamma_1 M_2 &= 0 \\
i = 1 : \lambda_1 M_0 + 2M_1 + \mu_1 M_2 &= 6 \left(\mu_1 \frac{y_2 - y_1}{h_2^2} - \lambda_1 \frac{y_1 - y_0}{h_1^2} \right) \\
M_0 - M_1(1 + \gamma_1) + \gamma_1 M_2 &= 0 \Big| \times \lambda_1 \\
M_2(\mu_1 \gamma_1^2 - \mu_1) - M_1(\lambda_1 + \lambda_1 \gamma_1 + 2) &= -6 \left(\mu_1 \frac{y_2 - y_1}{h_2^2} - \lambda_1 \frac{y_1 - y_0}{h_1^2} \right) \\
- \lambda_1 - \lambda_1 \gamma_1 - 2 &= -\lambda_1(1 + \gamma_1) - 2 = -\frac{h_1}{h_2 + h_1} \frac{h_2 + h_1}{h_2} - 2 = -\gamma_1 - 2 \\
M_1(-\gamma_1 - 2) + M_2(\mu_1 \gamma_1^2 - \mu_1) &= \underbrace{-6 \left(\mu_1 \frac{y_2 - y_1}{h_2^2} - \lambda_1 \frac{y_1 - y_0}{h_1^2} \right)}_{\widehat{g}_1}
\end{aligned}$$

$$\begin{aligned}
b_{n-2} &= b_{n-1} \\
\frac{M_{n-1} - M_{n-2}}{h_{n-1}} &= \frac{M_n - M_{n-1}}{h_n} \Big| \times h_n \\
\gamma_n &= \frac{h_n}{h_{n-1}} \\
\gamma_n M_{n-2} - M_{n-1}(1 + \gamma_n) + M_n &= 0 \\
i = n-1 : \lambda_{n-1} M_{n-2} + 2M_{n-1} + \mu_{n-1} M_n &= 6 \left(\mu_{n-1} \frac{y_n - y_{n-1}}{h_n^2} - \lambda_{n-1} \frac{y_{n-1} - y_{n-2}}{h_{n-1}^2} \right) \\
\gamma_n M_{n-2} - M_{n-1}(1 + \gamma_n) + M_n &= 0 \Big| \times \mu_{n-1} \\
M_{n-2}(\lambda_{n-1} \gamma_n^2 - \lambda_{n-1}) - M_{n-1}(\mu_{n-1} \gamma_n + \mu_{n-1} + 2) &= -6 \left(\mu_{n-1} \frac{y_n - y_{n-1}}{h_n^2} \right. \\
&\quad \left. - \lambda_{n-1} \frac{y_{n-1} - y_{n-2}}{h_{n-1}^2} \right) \\
- \mu_{n-1} - \mu_{n-1} \gamma_n - 2 &= \mu_{n-1}(1 + \gamma_n) - 2 = -\frac{h_n}{h_n + h_{n-1}} \frac{h_n + h_{n-1}}{h_{n-1}} - 2 = -\gamma_n - 2 \\
M_{n-2}(\lambda_{n-1} \gamma_n^2 - \lambda_{n-1}) + M_{n-1}(-\gamma_n - 2) &= \underbrace{-6 \left(\mu_{n-1} \frac{y_n - y_{n-1}}{h_n^2} - \lambda_{n-1} \frac{y_{n-1} - y_{n-2}}{h_{n-1}^2} \right)}_{\widehat{g}_{n-1}}
\end{aligned}$$

$$\begin{pmatrix}
-\gamma_1 - 2 & \mu_1 \gamma_1^2 - \mu_1 & 0 & 0 & \cdots & 0 & 0 & 0 \\
\lambda_2 & 2 & \mu_2 & 0 & \cdots & 0 & 0 & 0 \\
0 & \lambda_3 & 2 & \mu_3 & \cdots & 0 & 0 & 0 \\
\vdots & \vdots & \vdots & \vdots & \ddots & \vdots & \vdots & \vdots \\
0 & 0 & 0 & 0 & \cdots & \lambda_{n-2} & 2 & \mu_{n-2} \\
0 & 0 & 0 & 0 & \cdots & 0 & \lambda_{n-1} \gamma_n^2 - \lambda_{n-1} & -\gamma_n - 2
\end{pmatrix}
\begin{pmatrix}
M_1 \\
M_2 \\
M_3 \\
\vdots \\
M_{n-2} \\
M_{n-1}
\end{pmatrix}
=
\begin{pmatrix}
\widehat{g}_1 \\
g_2 \\
g_3 \\
\vdots \\
g_{n-2} \\
\widehat{g}_{n-1}
\end{pmatrix}$$